Revised to use modern proof technology, and also to flesh out the Hoare logic.

examples/ind_def/opsemScript.sml
@@ -1,167 +1,111 @@
-(* =====================================================================*)
-(* FILE		: opsemScript.sml					*)
-(* DESCRIPTION   : Creates a theory of the syntax and operational 	*)
-(* 		  semantics of a very simple imperative programming 	*)
-(* 		  language.  Illustrates the inductive definitions 	*)
-(* 		  package with proofs that the evaluation relation for	*)
-(*		  the given semantics is deterministic and that the 	*)
-(*		  Hoare-logic rule for while loops follows from a 	*)
-(*		  suitable definition of partial correctness.		*)
-(*									*)
-(* AUTHORS	: Tom Melham and Juanito Camilleri			*)
-(* DATE		: 91.10.09						*)
-(* TRANSLATED   : Dec. 27, 1992 Konrad Slind                            *)
-(* =====================================================================*)
-
-(* Interactive prelude
-  app load ["stringLib", "bossLib"];
-*)
-
+(*===========================================================================*)
+(* Operational semantics and program logic for a very simple imperative      *)
+(* programming language. Adapted from an example of Tom Melham and Juanito   *)
+(* Camilleri.                                                                *)
+(*===========================================================================*)
 
 structure opsemScript =
 struct
 
-open HolKernel Parse boolLib stringLib bossLib IndDefLib IndDefRules;
+(* Interactive use:
+  app load ["stringLib", "finite_mapTheory"];
+*)
 
-(* ---------------------------------------------------------------------*)
-(* Open a new theory and load the required libraries.			*)
-(* ---------------------------------------------------------------------*)
+open HolKernel Parse boolLib bossLib 
+     stringLib IndDefLib IndDefRules finite_mapTheory;
 
 val _ = new_theory "opsem";
 
-(* ===================================================================== *)
-(* Syntax of the programming language.					 *)
-(* ===================================================================== *)
+(*---------------------------------------------------------------------------*)
+(* Syntax of the programming language.					     *)
+(*                                                                           *)
+(* Program variables are represented by strings, and states are modelled by  *)
+(* finite maps from program variables to natural numbers.	             *)
+(*---------------------------------------------------------------------------*)
 
-(* --------------------------------------------------------------------- *)
-(* Program variables will be represented by strings, and states will be  *)
-(* modelled by functions from program variables to natural numbers.	 *)
-(* --------------------------------------------------------------------- *)
+val _ = type_abbrev("state", ``:string |-> num``);
 
-val state = Type`:string->num`;
+(*---------------------------------------------------------------------------*)
+(* Natural number expressions and boolean expressions are defined by         *)
+(* datatypes with simple evaluation semantics. In the following proofs,      *)
+(* neval and beval don't end up playing a role.                              *)
+(*---------------------------------------------------------------------------*)
 
-(* --------------------------------------------------------------------- *)
-(* Natural number expressions and boolean expressions will just be 	 *)
-(* modelled by total functions from states to numbers and booleans       *)
-(* respectively.  This simplification allows us to concentrate in this   *)
-(* example on defining the semantics of commands.			 *)
-(* --------------------------------------------------------------------- *)
+val _ = 
+ Hol_datatype 
+      `nexp = Var of string 
+            | Const of num
+            | Plus of nexp => nexp
+            | Times of nexp => nexp
+            | Sub of nexp => nexp`;
 
-val nexp = Type`:^state -> num`;
-val bexp = Type`:^state -> bool`;
+val _ = 
+ Hol_datatype 
+      `bexp = Equal of nexp => nexp
+            | Less of nexp => nexp
+            | Not of bexp`;
 
-(*---------------------------------------------------------------------------
-     Lift type antiquotes so they can be used in term quotations.
- ---------------------------------------------------------------------------*)
+val neval_def =  
+ Define
+  `(neval (Var s) sigma = (sigma ' s)) /\
+   (neval (Const c) sigma = c) /\
+   (neval (Plus e1 e2) sigma = neval e1 sigma + neval e2 sigma) /\
+   (neval (Times e1 e2) sigma = neval e1 sigma * neval e2 sigma) /\
+   (neval (Sub e1 e2) sigma = neval e1 sigma - neval e2 sigma)`;
 
-val State = ty_antiq state;
-val Bexp  = ty_antiq bexp;
+val beval_def =  
+ Define
+  `(beval (Equal e1 e2) sigma = (neval e1 sigma = neval e2 sigma)) /\
+   (beval (Less e1 e2) sigma = (neval e1 sigma < neval e2 sigma)) /\
+   (beval (Not e) sigma = ~(beval e sigma))`;
 
-(* ---------------------------------------------------------------------*)
-(* We can now use the recursive types package to define the syntax of   *)
-(* commands (or "programs').  We have the following types of commands:  *)
-(*									*)
-(*    C ::=   skip                     (does nothing)			*)
-(*          | V := E                   (assignment)          		*)
-(*          | C1 ; C2                  (sequencing)           		*)
-(*          | if B then C1 else C2     (conditional)			*)
-(*          | While B do C             (repetition)			*)
-(*                                                                      *)
-(* where V ranges over program variables, E ranges over natural number	*)
-(* expressions, B ranges over boolean expressions, and C, C1 and C2     *)
-(* range over commands.  						*)
-(*									*)
-(* In the logic, we represent this abstract syntax with a set of prefix *)
-(* type constructors. So we have:					*)
-(*						                        *)
-(*    V := E                  represented by `assign V E`		*)
-(*    C1 ; C2                 represented by `seq C1 C2`		*)
-(*    if B then C1 else C2    represented by `if B C1 C2`		*)
-(*    While B do C            represented by `While B C`		*)
-(*									*)
-(* ---------------------------------------------------------------------*)
 
-val _ = Hol_datatype
-          `comm
-             = Skip
-             | ::=    of string => ^nexp
-             | ;;    of  comm => comm
-             | If    of ^bexp => comm => comm
-             | While of ^bexp => comm`;
+(*---------------------------------------------------------------------------*)
+(* Datatype of programs                                                      *)
+(*---------------------------------------------------------------------------*)
 
-val _ = (set_fixity "::=" (Infixr 400); set_MLname "::=" "assign_def");
-val _ = (set_fixity ";;"  (Infixr 350); set_MLname ";;"  "seq_def");
+val _ = 
+ Hol_datatype
+  `program = Skip
+           | Assign of string => nexp
+           | Seq    of program => program
+           | Cond   of bexp => program => program
+           | While  of bexp => program`;
 
-(* ===================================================================== *)
-(* Definition of the operational semantics.				 *)
-(* ===================================================================== *)
 
-(* ---------------------------------------------------------------------*)
-(* The semantics of commands will be given by an evaluation relation	*)
-(*									*)
-(*       EVAL : comm -> state -> state -> bool     			*)
-(*									*)
-(* defined inductively such that 					*)
-(*									*)
-(*       EVAL C s1 s2							*)
-(*									*)
-(* holds exactly when executing the command C in the initial state s1 	*)
-(* terminates in the final state s2. The evaluation relation is defined *)
-(* inductively by the set of rules shown below.  			*)
-(* ---------------------------------------------------------------------*)
+(*---------------------------------------------------------------------------*)
+(* Operational semantics. The semantics of commands will be given by a       *)
+(* relation                                                                  *)
+(*                                                                           *)
+(*   EVAL : program -> state -> state -> bool                                *)
+(*                                                                           *)
+(* defined inductively such that                                             *)
+(*                                                                           *)
+(*   EVAL c s1 s2                                                            *)
+(*                                                                           *)
+(* holds exactly when executing the command c in the initial state s1        *)
+(* terminates in the final state s2. The evaluation relation is defined      *)
+(* inductively by the set of rules shown below.                              *)
+(*---------------------------------------------------------------------------*)
 
 val (rules,induction,ecases) = Hol_reln
-     `(!s. EVAL Skip s s)
- /\   (!s V E. EVAL (V ::= E) s (\v. if v=V then E s else s v))
- /\   (!C1 C2 s1 s3.
-        (?s2. EVAL C1 s1 s2 /\ EVAL C2 s2 s3) ==> EVAL (C1;;C2) s1 s3)
- /\   (!C1 C2 s1 s2 B. EVAL C1 s1 s2 /\  B s1 ==> EVAL (If B C1 C2) s1 s2)
- /\   (!C1 C2 s1 s2 B. EVAL C2 s1 s2 /\ ~B s1 ==> EVAL (If B C1 C2) s1 s2)
- /\   (!C s B.                           ~B s ==> EVAL (While B C) s s)
- /\   (!C s1 s3 B.
-        (?s2. EVAL C s1 s2 /\
-              EVAL (While B C) s2 s3 /\ B s1) ==> EVAL (While B C) s1 s3)`;
+   `(!s. EVAL Skip s s)
+ /\ (!s v e. EVAL (Assign v e) s (s |+ (v,neval e s)))
+ /\ (!c1 c2 s1 s2 s3. EVAL c1 s1 s2 /\ EVAL c2 s2 s3 ==> EVAL (Seq c1 c2) s1 s3)
+ /\ (!c1 c2 s1 s2 b.  EVAL c1 s1 s2 /\ beval b s1 ==> EVAL (Cond b c1 c2) s1 s2)
+ /\ (!c1 c2 s1 s2 b. EVAL c2 s1 s2 /\ ~beval b s1 ==> EVAL (Cond b c1 c2) s1 s2)
+ /\ (!c s b. ~beval b s ==> EVAL (While b c) s s)
+ /\ (!c s1 s2 s3 b.
+         EVAL c s1 s2 /\
+         EVAL (While b c) s2 s3 /\ beval b s1 ==> EVAL (While b c) s1 s3)`;
 
 val rulel = CONJUNCTS rules;
-
-(*---------------------------------------------------------------------------
-      Note that the following input is also acceptable to the
-      definition package (existentials on the left of implications
-      have been made into universals). This is in some way
-      cleaner, but some of the following proofs depend on the
-      specific structure of formulas and therefore fail with the
-      different representation.
-
-       (!s. EVAL Skip s s)
-   /\  (!s V E. EVAL (V ::= E) s (\v. if v=V then E s else s v))
-   /\  (!C1 C2 s1 s2 s3.
-                EVAL C1 s1 s2 /\ EVAL C2 s2 s3 ==> EVAL (C1;;C2) s1 s3)
-   /\  (!C1 C2 s1 s2 B. EVAL C1 s1 s2 /\  B s1 ==> EVAL (If B C1 C2) s1 s2)
-   /\  (!C1 C2 s1 s2 B. EVAL C2 s1 s2 /\ ~B s1 ==> EVAL (If B C1 C2) s1 s2)
-   /\  (!C s B.                           ~B s ==> EVAL (While B C) s s)
-   /\  (!C s1 s2 s3 B. EVAL C s1 s2 /\
-                EVAL (While B C) s2 s3 /\ B s1 ==> EVAL (While B C) s1 s3)
- ---------------------------------------------------------------------------*)
-
 
 (* --------------------------------------------------------------------- *)
 (* Stronger form of rule induction.					 *)
 (* --------------------------------------------------------------------- *)
 
-val sind = derive_strong_induction(rules,induction);
-
-(* ---------------------------------------------------------------------*)
-(* Construct the standard rule induction tactic for EVAL.  This uses	*)
-(* the "weaker' form of the rule induction theorem, and both premisses	*)
-(* and side conditions are simply assumed (in stripped form).  This 	*)
-(* served for many proofs, but when a more elaborate treatment of	*)
-(* premisses or side conditions is needed, or when the stronger form of	*)
-(* induction is required, a specialized  rule induction tactic is	*)
-(* constructed on the fly.						*)
-(* ---------------------------------------------------------------------*)
-
-val RULE_INDUCT_TAC =
-    RULE_INDUCT_THEN induction STRIP_ASSUME_TAC STRIP_ASSUME_TAC;
+val sinduction = derive_strong_induction(rules,induction);
 
 (* =====================================================================*)
 (* Derivation of backwards case analysis theorems for each rule.        *)
@@ -169,351 +113,173 @@ val RULE_INDUCT_TAC =
 (* These theorems are consequences of the general case analysis theorem *)
 (* proved above.  They are used to justify formal reasoning in which the*)
 (* rules are driven "backwards', inferring premisses from conclusions.  *)
-(* One infers from the assertion that:					*)
-(*									*)
-(*    1: EVAL C s1 s2 							*)
-(*									*)
-(* for a specific command C (e.g. for C = (--`Skip`--)) that the        *)
-(* corresponding instance of the premisses of the rule(s) for C must    *)
-(* also hold, since  (1) can hold only by virtue of being derivable by  *)
-(* the rule for C. This kind of reasoning occurs frequently in proofs   *)
-(* about operational semantics.  Formally, one must use the fact that   *)
-(* the logical representations of syntactically different commands are  *)
-(* distinct, a fact automatically proved by the recursive types package.*)
 (* =====================================================================*)
 
-(* ---------------------------------------------------------------------*)
-(* The following rule is used to simplify special cases of the general  *)
-(* exhaustive case analysis theorem, which looks something like:	*)
-(*									*)
-(*      |- !C s1 s2.							*)
-(*          EVAL C s1 s2 =						*)
-(*             (C = Skip) ... \/					*)
-(*             (?V E. (C = V ::= E) ...) \/				*)
-(*             (?C1 C2 s2'. (C = C1 ; C2) ...) \/			*)
-(*             (?C1 B C2. (C = If B C1 C2) /\ B s1 ...) \/		*)
-(*             (?C2 B C1. (C = If B C1 C2) /\ ~B s1 ...) \/		*)
-(*             (?B C'. (C = While B C') /\ ~B s1 ... ) \/		*)
-(*             (?C' B s2'. (C = While B C') /\ B s1 ...)		*)
-(*  									*)
-(* If C is specialized to some particular syntactic form, for example   *)
-(* to `C1;;C2`, then most of the disjuncts in the conclusion become     *)
-(* just false because of the syntactic inequality of different commands.*)
-(* These false can be simplified away by rewriting with the theorem	*)
-(* distinct.  The disjuncts that match the command to which C is 	*)
-(* specialized can also be simplified by rewriting with const11.  This  *)
-(* changes equalities between similar commands, for example:		*)
-(*									*)
-(*    (C1 ;; C2) = (C1' ;; C2')						*)
-(*									*)
-(* to equalities between their coresponding constitutents:		*)
-(*									*)
-(*    C1 = C1'  /\  C2 = C2'						*)
-(*									*)
-(* These can then generally be used for substitution.			*)
-(* ---------------------------------------------------------------------*)
+val SKIP_THM = store_thm
+("SKIP_THM",
+ ``!s1 s2. EVAL Skip s1 s2 = (s1 = s2)``,
+ RW_TAC std_ss [EQ_IMP_THM,Once ecases] THEN METIS_TAC rulel);
 
-val (distinct,const11) =
-  let val (SOME facts) = TypeBase.read {Thy="opsem", Tyop="comm"}
-      val thm1 = TypeBase.distinct_of ``:comm``
-      val thm2 = TypeBase.one_one_of ``:comm``
-  in
-    (CONJ thm1 (GSYM thm1),thm2)
-  end;
+val ASSIGN_THM = store_thm 
+("ASSIGN_THM",
+ ``!s1 s2 v e. EVAL (Assign v e) s1 s2 = (s2 = s1 |+ (v,neval e s1))``,
+ RW_TAC std_ss [EQ_IMP_THM,Once ecases] THEN METIS_TAC rulel);
 
-val SIMPLIFY = REWRITE_RULE [distinct, const11];
+val SEQ_THM = store_thm
+("SEQ_THM",
+ ``!s1 s3 c1 c2. EVAL (Seq c1 c2) s1 s3 = ?s2. EVAL c1 s1 s2 /\ EVAL c2 s2 s3``,
+ RW_TAC std_ss [EQ_IMP_THM,Once ecases] THEN METIS_TAC rulel);
 
-(* --------------------------------------------------------------------- *)
-(* CASE_TAC : this is applicable to goals of the form:			 *)
-(*									 *)
-(*      TRANS C s1 s2 ==> P						 *)
-(*									 *)
-(* When applied to such a goal, the antecedant is matched to the general *)
-(* case analysis theorem and a corresponding instance of its conclusion  *)
-(* is obtained.  This is simplified using the SIMPLIFY rule described    *)
-(* above and the result is assumed in stripped form.  Given this tactic, *)
-(* the sequence of theorems given below are simple to prove.  The proofs *)
-(* are fairly uniform; with a careful analysis of the regularities, one  *)
-(* should be able to devise an automatic proof procedure for deriving    *)
-(* sets of theorems of this type.					 *)
-(* --------------------------------------------------------------------- *)
+val IF_T_THM = store_thm 
+("IF_T_THM",
+ ``!s1 s2 b c1 c2. 
+     beval b s1 ==> (EVAL (Cond b c1 c2) s1 s2 = EVAL c1 s1 s2)``,
+ RW_TAC std_ss [EQ_IMP_THM,Once ecases] THEN METIS_TAC rulel);
 
-val CASE_TAC = DISCH_THEN
-               (STRIP_ASSUME_TAC o SIMPLIFY o ONCE_REWRITE_RULE[ecases]);
+val IF_F_THM = store_thm 
+("IF_F_THM",
+ ``!s1 s2 b c1 c2. 
+     ~beval b s1 ==> (EVAL (Cond b c1 c2) s1 s2 = EVAL c2 s1 s2)``,
+ RW_TAC std_ss [EQ_IMP_THM,Once ecases] THEN METIS_TAC rulel);
 
-(* --------------------------------------------------------------------- *)
-(* SKIP_THM : EVAL Skip s1 s2 is provable only by the Skip rule, which   *)
-(* requires that s1 and s2 be the same state.				 *)
-(* --------------------------------------------------------------------- *)
+val WHILE_T_THM = store_thm 
+("WHILE_T_THM",
+ ``!s1 s3 b c.
+    beval b s1 ==> 
+      (EVAL (While b c) s1 s3 = ?s2. EVAL c s1 s2 /\ 
+                                     EVAL (While b c) s2 s3)``,
+ RW_TAC std_ss [EQ_IMP_THM,Once ecases] THEN METIS_TAC rulel);
 
-val SKIP_THM = store_thm("SKIP_THM",
-     (--`!s1 s2. EVAL Skip s1 s2 = (s1 = s2)`--),
-     REPEAT GEN_TAC THEN EQ_TAC THENL
-     [CASE_TAC THEN ASM_REWRITE_TAC [],
-      DISCH_THEN SUBST1_TAC THEN MAP_FIRST RULE_TAC rulel]);
+val WHILE_F_THM = store_thm 
+("WHILE_F_THM",
+ ``!s1 s2 b c. ~beval b s1 ==> (EVAL (While b c) s1 s2 = (s1 = s2))``,
+ RW_TAC std_ss [EQ_IMP_THM,Once ecases] THEN METIS_TAC rulel);
+
+(*---------------------------------------------------------------------------*)
+(* THEOREM: the operational semantics is deterministic.                      *)
+(*                                                                           *)
+(* Given the suite of theorems proved above, this proof is relatively        *)
+(* straightforward.  The standard proof is by structural induction on c, but *)
+(* the proof by rule induction given below gives rise to a slightly easier   *)
+(* analysis in each case of the induction.  There are, however, more         *)
+(* cases---one per rule, rather than one per constructor.                    *)
+(*---------------------------------------------------------------------------*)
+
+val EVAL_DETERMINISTIC = store_thm 
+("EVAL_DETERMINISTIC",
+ ``!c st1 st2. EVAL c st1 st2 ==> !st3. EVAL c st1 st3 ==> (st2 = st3)``,
+ HO_MATCH_MP_TAC induction THEN 
+ RW_TAC std_ss [SKIP_THM,ASSIGN_THM,SEQ_THM,
+                IF_T_THM,IF_F_THM,WHILE_T_THM, WHILE_F_THM] THEN 
+ METIS_TAC[]);
+
+(*---------------------------------------------------------------------------*)
+(* Definition of Floyd-Hoare logic judgements for partial correctness and    *)
+(* derivation of proof rules.                                                *)
+(*---------------------------------------------------------------------------*)
+
+val SPEC_def = 
+ Define 
+   `SPEC P c Q = !s1 s2. P s1 /\ EVAL c s1 s2 ==> Q s2`;
 
 
-(* --------------------------------------------------------------------- *)
-(* ASSIGN_THM : EVAL (V ::= E) s1 s2 is provable only by the assignment	 *)
-(* rule, which requires that s2 be the state s1 with V updated to E.	 *)
-(* --------------------------------------------------------------------- *)
+(*---------------------------------------------------------------------------*)
+(* Skip rule                                                                 *)
+(*---------------------------------------------------------------------------*)
 
-val ASSIGN_THM = store_thm ("ASSIGN_THM",
- (--`!s1 s2 V E. EVAL (V ::= E) s1 s2
-                   =
-                 ((\v. if v=V then E s1 else s1 v) = s2)`--),
-     REPEAT GEN_TAC THEN EQ_TAC THENL
-     [CASE_TAC THEN ASM_REWRITE_TAC [],
-      DISCH_THEN (SUBST1_TAC o SYM) THEN MAP_FIRST RULE_TAC rulel]);
+val SKIP_RULE = store_thm
+("SKIP_RULE",
+ ``!P. SPEC P Skip P``,
+ RW_TAC std_ss [SPEC_def,SKIP_THM]);
 
+(*---------------------------------------------------------------------------*)
+(* Assignment rule                                                           *)
+(*---------------------------------------------------------------------------*)
 
-(* --------------------------------------------------------------------- *)
-(* SEQ_THM : EVAL (C1;;C2) s1 s2 is provable only by the sequencing      *)
-(* rule, which requires that some intermediate state s3 exists such      *)
-(* that C1 in state s1 terminates in s3 and C3 in s3 terminates in s2.   *)
-(* --------------------------------------------------------------------- *)
+val ASSIGN_RULE = store_thm
+("ASSIGN_RULE",
+ ``!P v e.
+      SPEC (\s. P (s |+ (v,neval e s))) (Assign v e) P``,
+ RW_TAC std_ss [SPEC_def] THEN METIS_TAC [ASSIGN_THM]);
 
-val SEQ_THM = store_thm("SEQ_THM",
---`!s1 s2 C1 C2.EVAL (C1;;C2) s1 s2 = ?s3. EVAL C1 s1 s3 /\ EVAL C2 s3 s2`--,
-  REPEAT GEN_TAC THEN EQ_TAC THENL
-  [CASE_TAC THEN EXISTS_TAC (--`s2':^State`--) THEN ASM_REWRITE_TAC [],
-   DISCH_THEN (fn th => MAP_FIRST RULE_TAC rulel THEN MATCH_ACCEPT_TAC th)]);
+(*---------------------------------------------------------------------------*)
+(* Sequencing rule                                                           *)
+(*---------------------------------------------------------------------------*)
 
+val SEQ_RULE = store_thm
+("SEQ_RULE",
+ ``!P c1 c2 Q R. 
+       SPEC P c1 Q /\ SPEC Q c2 R ==> SPEC P (Seq c1 c2) R``,
+ RW_TAC std_ss [SPEC_def] THEN METIS_TAC [SEQ_THM]);
 
-(* --------------------------------------------------------------------- *)
-(* IF_T_THM : if B(s1) is true, then EVAL (If B C2 C2) s1 s2 is provable *)
-(* only by the first conditional rule, which requires that C1 when	 *)
-(* evaluated in s1 terminates in s2.					 *)
-(* --------------------------------------------------------------------- *)
+(*---------------------------------------------------------------------------*)
+(* Conditional rule                                                          *)
+(*---------------------------------------------------------------------------*)
 
-val IF_T_THM = store_thm ("IF_T_THM",
-(--`!s1 s2 B C1 C2. B s1 ==> (EVAL (If B C1 C2) s1 s2 = EVAL C1 s1 s2)`--),
-     REPEAT STRIP_TAC THEN EQ_TAC THENL
-     [CASE_TAC THEN EVERY_ASSUM (TRY o SUBST_ALL_TAC) THENL
-      [FIRST_ASSUM ACCEPT_TAC, RES_TAC],
-      DISCH_TAC THEN MAP_FIRST RULE_TAC rulel THEN FIRST_ASSUM ACCEPT_TAC]);
+val COND_RULE = store_thm
+("COND_RULE",
+ ``!P b c1 c2 Q.
+      SPEC (\s. P(s) /\ beval b s) c1 Q /\ 
+      SPEC (\s. P(s) /\ ~beval b s) c2 Q ==> SPEC P (Cond b c1 c2) Q``,
+ RW_TAC std_ss [SPEC_def] THEN METIS_TAC [IF_T_THM, IF_F_THM]);
 
+(*---------------------------------------------------------------------------*)
+(* While rule                                                                *)
+(*---------------------------------------------------------------------------*)
 
-(* --------------------------------------------------------------------- *)
-(* IF_F_THM : if B(s1) is false, then EVAL (if B C1 C2) s1 s2 is 	 *)
-(* provable only by the second conditional rule, which requires that C2	 *)
-(* when evaluated in s1 terminates in s2.				 *)
-(* --------------------------------------------------------------------- *)
+val lemma1 = Q.prove
+(`!c s1 s2. EVAL c s1 s2 ==> !b' c'. (c = While b' c') ==> ~beval b' s2`,
+ HO_MATCH_MP_TAC induction THEN RW_TAC std_ss []);
 
-val IF_F_THM = store_thm ("IF_F_THM",
-(--`!s1 s2 B C1 C2. ~B s1 ==> (EVAL (If B C1 C2) s1 s2 = EVAL C2 s1 s2)`--),
-   REPEAT STRIP_TAC THEN EQ_TAC THENL
-   [CASE_TAC THEN EVERY_ASSUM (TRY o SUBST_ALL_TAC) THENL
-    [RES_TAC, FIRST_ASSUM ACCEPT_TAC],
-     DISCH_TAC THEN MAP_FIRST RULE_TAC (rev rulel) THEN
-     FIRST_ASSUM ACCEPT_TAC]);
+val lemma2 = Q.prove
+(`!c s1 s2.
+   EVAL c s1 s2 ==>
+     !b' c'. (c = While b' c') ==>
+             (!s1 s2. P s1 /\ beval b' s1 /\ EVAL c' s1 s2 ==> P s2) ==>
+             (P s1 ==> P s2)`,
+ HO_MATCH_MP_TAC sinduction THEN RW_TAC std_ss [] THEN METIS_TAC[]);
 
-
-(* ---------------------------------------------------------------------*)
-(* WHILE_T_THM : if B(s1) is true, then EVAL (While B C) s1 s2 is 	*)
-(* provable only by the corresponding While rule, which requires that 	*)
-(* there is an intermediate state s3 such that C in state s1 terminates *)
-(* in s3, and While B do C in state s3 terminates in s2.		*)
-(* ---------------------------------------------------------------------*)
-
-val WHILE_T_THM = store_thm ("WHILE_T_THM",
-     (--`!s1 s2 B C.
-      B s1 ==> (EVAL (While B C) s1 s2 =
-                (?s3. EVAL C s1 s3 /\ EVAL (While B C) s3 s2))`--),
-   REPEAT STRIP_TAC THEN EQ_TAC THENL
-   [CASE_TAC THEN EVERY_ASSUM (TRY o SUBST_ALL_TAC) THENL
-    [RES_TAC,
-     EXISTS_TAC (--`s2':^State`--) THEN CONJ_TAC THEN FIRST_ASSUM ACCEPT_TAC],
-    STRIP_TAC THEN MAP_FIRST RULE_TAC (rev rulel) THEN
-    EXISTS_TAC (--`s3:^State`--) THEN
-    REPEAT CONJ_TAC THEN FIRST_ASSUM ACCEPT_TAC]);
+val WHILE_RULE = store_thm
+("WHILE_RULE",
+ ``!P b c. SPEC (\s. P(s) /\ beval b s) c P ==>
+           SPEC P (While b c) (\s. P s /\ ~beval b s)``,
+ RW_TAC std_ss [SPEC_def] THENL [METIS_TAC[lemma2],METIS_TAC[lemma1]]);
 
 
-(* ---------------------------------------------------------------------*)
-(* WHILE_F_THM : if B(s1) is false, then EVAL (While B C) s1 s2 is	*)
-(* provable only by the corresponding While rule, which requires that 	*)
-(* s2 equals the original state s1					*)
-(* ---------------------------------------------------------------------*)
+(*---------------------------------------------------------------------------*)
+(* Precondition strengthening                                                *)
+(*---------------------------------------------------------------------------*)
 
-val WHILE_F_THM = store_thm ("WHILE_F_THM",
-     (--`!s1 s2 B C. ~B s1 ==> (EVAL (While B C) s1 s2 = (s1 = s2))`--),
-     REPEAT STRIP_TAC THEN EQ_TAC THENL
-     [CASE_TAC THENL
-      [CONV_TAC SYM_CONV THEN FIRST_ASSUM ACCEPT_TAC,
-       EVERY_ASSUM (TRY o SUBST_ALL_TAC) THEN RES_TAC],
-      DISCH_THEN (SUBST1_TAC o SYM) THEN MAP_FIRST RULE_TAC rulel THEN
-      FIRST_ASSUM ACCEPT_TAC]);
+val PRE_STRENGTHEN = store_thm
+("PRE_STRENGTHEN",
+ ``!P c Q P'. (!s. P' s ==> P s) /\  SPEC P c Q ==> SPEC P' c Q``,
+ RW_TAC std_ss [SPEC_def] THEN METIS_TAC[]);
 
+(*---------------------------------------------------------------------------*)
+(* postcondition weakening                                                   *)
+(*---------------------------------------------------------------------------*)
 
-(* ===================================================================== *)
-(* THEOREM: the operational semantics is deterministic.			 *)
-(*									 *)
-(* Given the suite of theorems proved above, this proof is relatively    *)
-(* strightforward.  The standard proof is by structural induction on C,  *)
-(* but the proof by rule induction given below gives rise to a slightly  *)
-(* easier analysis in each case of the induction.  There are, however,   *)
-(* more cases---one per rule, rather than one per constructor.		 *)
-(* ===================================================================== *)
+val POST_WEAKEN = store_thm
+("POST_WEAKEN",
+ ``!P c Q Q'. (!s. Q s ==> Q' s) /\  SPEC P c Q ==> SPEC P c Q'``,
+ RW_TAC std_ss [SPEC_def] THEN METIS_TAC[]);
 
-val DETERMINISTIC = store_thm ("DETERMINISTIC",
-(--`!C st1 st2. EVAL C st1 st2 ==> !st3. EVAL C st1 st3 ==> (st2 = st3)`--),
-     RULE_INDUCT_TAC THEN REPEAT GEN_TAC THENL
-     [REWRITE_TAC [SKIP_THM],
-      REWRITE_TAC [ASSIGN_THM],
-      PURE_ONCE_REWRITE_TAC [SEQ_THM] THEN STRIP_TAC THEN
-      FIRST_ASSUM MATCH_MP_TAC THEN RES_TAC THEN ASM_REWRITE_TAC [],
-      IMP_RES_TAC IF_T_THM THEN ASM_REWRITE_TAC [],
-      IMP_RES_TAC IF_F_THM THEN ASM_REWRITE_TAC [],
-      IMP_RES_TAC WHILE_F_THM THEN ASM_REWRITE_TAC [],
-      IMP_RES_THEN (fn th =>  PURE_ONCE_REWRITE_TAC [th]) WHILE_T_THM THEN
-      STRIP_TAC THEN FIRST_ASSUM MATCH_MP_TAC THEN
-      RES_TAC THEN ASM_REWRITE_TAC []]);
+(*---------------------------------------------------------------------------*)
+(* Boolean combinations of pre-and-post-conditions.                          *)
+(*---------------------------------------------------------------------------*)
 
+val CONJ_TRIPLE = store_thm
+("CONJ_TRIPLE",
+ ``!P1 P2 c Q1 Q2. SPEC P1 c Q1 /\ SPEC P2 c Q2 
+                   ==> SPEC (\s. P1 s /\ P2 s) c (\s. Q1 s /\ Q2 s)``,
+ RW_TAC std_ss [SPEC_def] THEN METIS_TAC[]);
 
-(* ===================================================================== *)
-(* Definition of partial correctness and derivation of proof rules.	 *)
-(* ===================================================================== *)
-
-val SPEC_DEF = new_definition ("SPEC_DEF",
-     (--`SPEC P C Q = !s1 s2. (P s1 /\ EVAL C s1 s2) ==> Q s2`--));
-
-(* --------------------------------------------------------------------- *)
-(* Proof of the While rule in Hoare logic.				 *)
-(* --------------------------------------------------------------------- *)
-
-(* --------------------------------------------------------------------- *)
-(* In the following proofs, theorems of the form:			 *)
-(*									 *)
-(*     |- !y1...yn. (C x1 ... xn = C y1 ... yn) ==> tm[y1,...,yn]	 *)
-(*									 *)
-(* frequently arise, where C is one of the constructors of the data type *)
-(* of commands.  The following theorem-tactic simplifies such theorems   *)
-(* by specializing yi to xi and then removing the resulting trivially    *)
-(* true antecedent.  The result is:					 *)
-(*									 *)
-(*     |- tm[x1,...,xn/y1,...,yn]					 *)
-(*									 *)
-(* which is passed to the theorem continuation function. The tactic just *)
-(* discards theorems not of the form shown above.   For the While proof  *)
-(* given below, this has the effect of thinning out useless induction	 *)
-(* hypotheses of the form:						 *)
-(*									 *)
-(*     |- !B' C'. (C = While B' C') ==> tm[B',C']			 *)
-(* 									 *)
-(* These are just discarded.						 *)
-(* --------------------------------------------------------------------- *)
-
-fun REFL_MP_THEN ttac th =
-   let val tm = lhs(fst(dest_imp(snd(strip_forall(concl th)))))
-   in ttac (MATCH_MP th (REFL tm))
-   end handle HOL_ERR _ => ALL_TAC;
-
-(* --------------------------------------------------------------------- *)
-(* The following lemma states that the condition B in While B C must be  *)
-(* false upon termination of a While loop.  The proof is by a rule 	 *)
-(* induction specialized to the While rule cases.  We show that the set	 *)
-(* 									 *)
-(*    {(While B C,s1,s2) | ~(B s2)} U {(C,s1,s2) | ~(C = While B' C')}   *)
-(*									 *)
-(* is closed under the rules for the evaluation relation. Note that this *)
-(* formulation illustrates a general way of proving a property of some   *)
-(* specific class of commands by rule induction.  One takes the union of *)
-(* the set containing triples with the desired property and the set of   *)
-(* all other triples whose command component is NOT an element of the    *)
-(* class of commands of interest.					 *)
-(*									 *)
-(* The proof is trivial for all but the two While rules, since this set	 *)
-(* contains all triples (C,s1,s2) for which C is not a While command.  	 *)
-(* The subgoals corresponding to these cases are vacuously true, since 	 *)
-(* they are implications with antecedents of the form (C = While B' C'), *)
-(* where C is a command syntactically distinct from any While command.	 *)
-(*									 *)
-(* Showing that the above set is closed under the two While rules is     *)
-(* likewise trivial.  For the While axiom, we get ~(B s2) immediately 	 *)
-(* from the side condition. For the other While rule, the statement to	 *)
-(* prove is just one of the induction hypotheses; since RULE_INDUCT_TAC  *)
-(* uses STRIP_ASSUME_TAC on this hypothesis, this subgoal is solved	 *)
-(* immediately.								 *)
-(* --------------------------------------------------------------------- *)
-
-
-val WHILE_LEMMA1 = TAC_PROOF(([],
- (--`!C s1 s2. EVAL C s1 s2 ==> !B' C'. (C = While B' C') ==> ~(B' s2)`--)),
-     RULE_INDUCT_TAC THEN REWRITE_TAC [distinct, const11] THEN
-     REPEAT GEN_TAC THEN DISCH_THEN (STRIP_THM_THEN SUBST_ALL_TAC) THEN
-     FIRST_ASSUM ACCEPT_TAC);
-
-(* ---------------------------------------------------------------------*)
-(* The second lemma deals with the invariant part of the Hoare proof 	*)
-(* rule for While commands.  We show that if P is an invariant of C, 	*)
-(* then it is also an invariant of While B C.  The proof is essentially *)
-(* an induction on the number of applications of the evaluation rule for*)
-(* While commands.  This is expressed as a rule induction, which 	*)
-(* establishes that the set:						*)
-(*									*)
-(*    {(While B C,s1,s2) | P invariant of C ==> (P s1 ==> P s2)}	*)
-(*									*)
-(* is closed under the transition rules.  As in lemma 1, the rules for  *)
-(* other kinds of commands are dealt with by taking the union of this 	*)
-(* set with 								*)
-(* 									*)
-(*    {(C,s1,s2) | ~(C = While B' C')}					*)
-(*									*)
-(* Closure under evaluation rules other than the two rules for While is *)
-(* therefore trivial, as outlined in the comments to lemma 1 above. 	*)
-(*									*)
-(* The proof in fact proceeds by strong rule induction.  With ordinary  *)
-(* rule induction, one obtains hypotheses that are too weak to imply the*)
-(* desired conclusion in the step case of the While rule.  To see why, 	*)
-(* try replacing strong by weak induction in the tactic proof below.	*)
-(*									*)
-(* Note that REFL_MP_THEN is used to simplify the induction hypotheses  *)
-(* before adding them to the assumption list.  This avoids having the 	*)
-(* assumptions in an awkward form (try using ASSUME_TAC instead). Note	*)
-(* also that in the case of the While axiom, the states s1 and s2 are	*)
-(* identical, so the corresponding subgoal is trivial and is solved by	*)
-(* the rewriting step.							*)
-(* ---------------------------------------------------------------------*)
-
-val WHILE_LEMMA2 =
-    TAC_PROOF(([],
-  --`!C s1 s2.
-     EVAL C s1 s2 ==>
-     !B' C'. (C = While B' C') ==>
-             (!s1 s2. P s1 /\ B' s1 /\ EVAL C' s1 s2 ==> P s2) ==>
-             (P s1 ==> P s2)`--),
-     RULE_INDUCT_THEN sind (REFL_MP_THEN ASSUME_TAC) ASSUME_TAC THEN
-     REWRITE_TAC [distinct, const11] THEN REPEAT GEN_TAC THEN
-     DISCH_THEN (STRIP_THM_THEN SUBST_ALL_TAC) THEN
-     REPEAT STRIP_TAC THEN RES_TAC);
-
-(* ---------------------------------------------------------------------*)
-(* The proof rule for While commands in Hoare logic is:			*)
-(*									*)
-(*         |- {P /\ B} C {P}						*)
-(*      ----------------------						*)
-(*        |- {P} C {P /\ ~B}						*)
-(* 									*)
-(* Given the two lemmas proved above, it is trivial to prove this rule. *)
-(* The antecedent of the rule is just the assumption of invariance of P *)
-(* for C which occurs in lemma 2.  Note that REFL_MP_THEN is used to    *)
-(* simplify the conclusions of the lemmas after one resolution step.	*)
-(* ---------------------------------------------------------------------*)
-
-val WHILE = store_thm ("WHILE",
-     (--`!P C. SPEC (\s. P s /\ B s) C P ==>
-            SPEC P (While B C) (\s. P s /\ ~B s)`--),
-     PURE_ONCE_REWRITE_TAC [SPEC_DEF] THEN
-     CONV_TAC (ONCE_DEPTH_CONV BETA_CONV) THEN
-     PURE_ONCE_REWRITE_TAC [SYM(SPEC_ALL CONJ_ASSOC)] THEN
-     REPEAT STRIP_TAC THENL
-     [IMP_RES_THEN (REFL_MP_THEN IMP_RES_TAC) WHILE_LEMMA2,
-      IMP_RES_THEN (REFL_MP_THEN IMP_RES_TAC) WHILE_LEMMA1]);
-
-(* ---------------------------------------------------------------------*)
-(* End of example.							*)
-(* ---------------------------------------------------------------------*)
+val DISJ_TRIPLE = store_thm
+("DISJ_TRIPLE",
+ ``!P1 P2 c Q1 Q2. SPEC P1 c Q1 /\ SPEC P2 c Q2 
+                   ==> SPEC (\s. P1 s \/ P2 s) c (\s. Q1 s \/ Q2 s)``,
+ RW_TAC std_ss [SPEC_def] THEN METIS_TAC[]);
 
 val _ = export_theory();
 
-end;
+end
